read_buf() function.

code/Yazi.LZ77.fst
@@ -1,8 +1,11 @@
 module Yazi.LZ77
 
+module Adler32 = Yazi.Adler32
 module B = LowStar.Buffer
 module Cast = FStar.Int.Cast
 module CB = LowStar.ConstBuffer
+module CFlags = Yazi.CFlags
+module CRC32 = Yazi.CRC32
 module ST = FStar.HyperStack.ST
 module U16 = FStar.UInt16
 module U32 = FStar.UInt32
@@ -11,6 +14,7 @@ module U8 = FStar.UInt8
 open LowStar.BufferOps
 open FStar.Mul
 open Spec.LZ77
+open Lib.Seq
 
 let context_valid (c: lz77_context) =
   let open U16 in
@@ -36,27 +40,54 @@ let update_hash
   ST.StackInline unit
   (ensures fun h ->
     let open U16 in
-    let ctx' = CB.as_mbuf ctx in
     CB.length ctx == 1 /\
-    (let ctx'' = B.get h ctx' 0 in
-    CB.live h ctx /\ B.live h ins_h /\
-    B.disjoint ctx' ins_h /\
-    context_valid ctx'' /\
-    is_rolling_hash (v ctx''.h_bits) a b c (B.get h ins_h 0)))
+    (let ctx' = B.get h (CB.as_mbuf ctx) 0 in
+    CB.live h ctx /\ B.live h ins_h /\ B.disjoint ins_h (CB.as_mbuf ctx) /\
+    context_valid ctx' /\
+    is_rolling_hash (v ctx'.h_bits) a b c (B.get h ins_h 0)))
   (requires fun h0 _ h1 ->
     let open U16 in
     let ctx' = B.get h1 (CB.as_mbuf ctx) 0 in
-    let h = B.get h1 ins_h 0 in
+    let hash = B.get h1 ins_h 0 in
     B.modifies (B.loc_buffer ins_h) h0 h1 /\
-    is_rolling_hash (v ctx'.h_bits) b c d h) =
+    is_rolling_hash (v ctx'.h_bits) b c d (B.get h1 ins_h 0)) =
   let open U16 in
-  let d' = Cast.uint8_to_uint16 d in
+  [@inline_let] let d' = Cast.uint8_to_uint16 d in
   let bits = (CB.index ctx 0ul).h_bits in
   let bits': Ghost.erased hash_bits = Ghost.hide (v bits) in
   let s = (CB.index ctx 0ul).shift in
   let m = (CB.index ctx 0ul).h_mask in
-  let s' = Cast.uint16_to_uint32 s in
-  let h = !*ins_h in
-  let h' = ((h <<^ s') ^^ d') &^ m in
-  roll_hash_eq bits' m s a b c d h;
-  ins_h *= h'
+  [@inline_let] let s' = Cast.uint16_to_uint32 s in
+  let hash = !*ins_h in
+  roll_hash_eq bits' m s a b c d hash;
+  ins_h *= (((hash <<^ s') ^^ d') &^ m)
+
+#set-options "--z3rlimit 200 --fuel 0 --ifuel 0"
+let read_buf ss uncompressed next_in buf size wrap =
+  let open U32 in
+  let avail_in = ss.(0ul) in
+  let len = if avail_in >^ size then
+    size
+  else
+    avail_in
+  in
+  [@inline_let] let avail_in' = B.sub ss 0ul 1ul in
+  let next_in' = !*next_in in
+  let ulen = Ghost.hide (Seq.length uncompressed) in
+    
+  B.blit next_in' 0ul buf 0ul len;
+  let buf' = B.sub next_in' 0ul (Ghost.hide len) in
+  if wrap = 1l then begin
+    ss.(4ul) <- (Adler32.adler32 #ulen (Ghost.reveal uncompressed) ss.(4ul) buf' len)
+  end else if CFlags.gzip then
+    if wrap = 2l then
+      ss.(4ul) <- (CRC32.crc32 uncompressed ss.(4ul) buf' len)
+    else
+      ()
+  else
+    ();
+  next_in *= (B.sub next_in' len (avail_in -^ len));
+  ss.(0ul) <- avail_in -^ len;
+  ss.(1ul) <- U32.add_underspec ss.(1ul) len;
+  (len, Ghost.hide buf')
+
