code/Yazi.LZ77.fsti
@@ -1,16 +1,24 @@
 module Yazi.LZ77
 
+module Adler32 = Spec.Adler32
 module B = LowStar.Buffer
+module CFlags = Yazi.CFlags
+module CRC32 = Spec.CRC32
+module HS = FStar.HyperStack
+module I32 = FStar.Int32
+module S = Spec.State
+module Seq = FStar.Seq
+module ST = FStar.HyperStack.ST
 module U16 = FStar.UInt16
 module U32 = FStar.UInt32
 module U8 = FStar.UInt8
+module Util = Yazi.Util
 
 noeq type lz77_context = {
   w_size: U32.t;        (* LZ77 window size (32K by default) *)
   w_bits: U16.t;        (* log2 w_size  (8..16) *)
   w_mask: U16.t;        (* w_size - 1 *)
 
-  window: B.buffer U8.t;
   (* Sliding window. Input bytes are read into the second half of the window,
    * and move to the first half later to keep a dictionary of at least wSize
    * bytes. With this organization, matches are limited to a distance of
@@ -18,10 +26,11 @@ noeq type lz77_context = {
    * performed with a length multiple of the block size. Also, it limits
    * the window size to 64K, which is quite useful on MSDOS.
    * To do: use the user input buffer as sliding window. *)
+  window: B.buffer U8.t;
 
-  window_size: U32.t;
   (* Actual size of window: 2 * w_size, except when the user input buffer
    * is directly used as sliding window. *)
+  window_size: U32.t;
      
   (* Link to older string with same hash index. To limit the size of this
    * array to 64K, this link is maintained only for the last 32K strings.
@@ -40,3 +49,66 @@ noeq type lz77_context = {
    *   shift * MIN_MATCH >=h_bits *)
   shift: U16.t;
 }
+
+noeq type lz77_state = {
+  (* Window position at the beginning of the current output block. Gets
+   * negative when the window is moved backwards. *)
+  block_start: I32.t;
+
+  ins_h: U32.t;        (* hash index of string to be inserted *)
+  match_length: U32.t; (* length of best match *)
+  prev_match: U32.t;   (* previous match *)
+  strstart: U32.t;     (* start of string to insert *)
+  match_start: U32.t;  (* start of matching string *)
+  lookahead: U32.t;    (* number of valid bytes ahead in window *)
+
+  (* Length of the best match at previous step. Matches not greater than this
+   * are discarded. This is used in the lazy match evaluation. *)
+  prev_length: U32.t;
+  match_available: bool; (* set if previous match exists *)
+}
+
+type stream_state = B.lbuffer U32.t 5
+
+val read_buf:
+    ss: stream_state
+  -> uncompressed: Ghost.erased (Seq.seq U8.t)
+  -> next_in: B.pointer (B.buffer U8.t)
+  -> buf: B.buffer U8.t
+  -> size: U32.t
+  -> wrap: I32.t
+  -> ST.Stack (U32.t & Ghost.erased (B.buffer U8.t))
+  (requires fun h -> 
+    let len = if U32.v size > S.avail_in (B.as_seq h ss) then
+      S.avail_in (B.as_seq h ss)
+    else
+      U32.v size
+    in
+    len > 0 /\
+    B.live h ss /\ ~(B.g_is_null ss) /\
+    B.live h buf /\ ~(B.g_is_null buf) /\
+    HS.disjoint (B.frameOf ss) (B.frameOf buf) /\
+    B.length buf == U32.v size /\
+    S.next_in_valid h ss next_in /\
+    S.adler_valid h ss wrap uncompressed)
+  (ensures fun h0 res h1 ->
+  let (len', read) = res in
+  let next_in0 = B.get h0 next_in 0 in
+  let next_in1 = B.get h1 next_in 0 in
+  let s0 = B.as_seq h0 ss in
+  let s1 = B.as_seq h1 ss in
+  let len = if U32.v size > S.avail_in s0 then
+    S.avail_in s0
+  else
+    U32.v size
+  in
+  len == U32.v len' /\
+  B.modifies (B.loc_union
+    (B.loc_buffer ss)
+    (B.loc_union (B.loc_buffer next_in) (B.loc_buffer buf))) h0 h1 /\
+  Seq.equal (B.as_seq h1 read) (B.as_seq h0 (B.gsub next_in0 0ul len')) /\
+  S.avail_in s0 - len == S.avail_in s1 /\
+  S.next_in_valid h1 ss next_in /\
+  S.adler_valid h1 ss wrap (Seq.append uncompressed (B.as_seq h1 read)) /\
+  S.avail_out s0 == S.avail_out s1 /\
+  S.total_out s0 == S.total_out s1)
