lib/Lib.Seq.fsti
@@ -10,3 +10,18 @@ let unsnoc (#a: Type) (s: Seq.seq a{
     Seq.index s i == Seq.index res i)
 }) =
   Seq.slice s 0 (Seq.length s - 1)
+
+unfold let op_String_Access #a = Seq.index #a
+
+let slice_empty (#a: Type) (s: Seq.seq a) (len: nat): Lemma
+  (requires len == 0)
+  (ensures Seq.slice s 0 len == Seq.empty #a /\ Seq.length (Seq.slice s 0 len) == 0)
+  [SMTPat (Seq.slice s 0 len)] =
+  Seq.lemma_empty (Seq.slice s 0 len)
+
+let append_empty_seq_r (#a: Type) (s1 s2: Seq.seq a): Lemma
+  (requires Seq.length s2 == 0)
+  (ensures Seq.append s1 s2 == s1)
+  [SMTPat (Seq.append s1 s2)] =
+  Seq.lemma_empty s2;
+  Seq.append_empty_r s1
