lib/Lib.Buffer.fsti
@@ -1,0 +1,14 @@
+module Lib.Buffer
+
+module B = LowStar.Buffer
+module HS = FStar.HyperStack
+module Seq = FStar.Seq
+
+let append_empty_buf_r (#a: Type) (h: HS.mem) (buf: B.buffer a) (s: Seq.seq a): Lemma
+  (requires B.length buf == 0)
+  (ensures Seq.append s (B.as_seq h buf) == s)
+  [SMTPat (Seq.append s (B.as_seq h buf))] =
+  assert(Seq.length (B.as_seq h buf) == 0);
+  Seq.lemma_empty (B.as_seq h buf);
+  Seq.append_empty_r s
+
