specs/Spec.State.fsti
@@ -1,0 +1,75 @@
+module Spec.State
+
+module Adler32 = Spec.Adler32
+module B = LowStar.Buffer
+module CFlags = Yazi.CFlags
+module CRC32 = Spec.CRC32
+module HS = FStar.HyperStack
+module I32 = FStar.Int32
+module Seq = FStar.Seq
+module U32 = FStar.UInt32
+module U8 = FStar.UInt8
+
+open Lib.Seq
+
+type stream_state = s:Seq.seq U32.t{Seq.length s == 5}
+
+unfold let avail_in (s: stream_state) = U32.v s.[0]
+unfold let total_in (s: stream_state) = U32.v s.[1]
+unfold let avail_out (s: stream_state) = U32.v s.[2]
+unfold let total_out (s: stream_state) = U32.v s.[3]
+unfold let adler (s: stream_state) = s.[4]
+
+unfold let next_in_valid
+  (h: HS.mem)
+  (s: B.lbuffer U32.t 5)
+  (next_in: B.pointer (B.buffer U8.t)) =
+  let next_in' = B.get h next_in 0 in
+  B.frameOf next_in == B.frameOf s /\
+  B.frameOf next_in' == B.frameOf s /\
+  B.live h next_in /\ B.live h next_in' /\
+  B.disjoint next_in s /\ B.disjoint next_in' s /\ B.disjoint next_in next_in' /\
+  B.length next_in' == avail_in (B.as_seq h s)
+
+unfold let next_out_valid
+  (h: HS.mem)
+  (s: B.lbuffer U32.t 5)
+  (next_out: B.pointer (B.buffer U8.t)) =
+  let next_out' = B.get h next_out 0 in
+  B.frameOf next_out == B.frameOf s /\
+  B.frameOf next_out' == B.frameOf s /\
+  B.live h next_out /\ B.live h next_out' /\
+  B.disjoint next_out s /\ B.disjoint next_out' s /\ B.disjoint next_out next_out' /\
+  B.length next_out' == avail_out (B.as_seq h s)
+
+unfold let adler_valid
+  (h: HS.mem)
+  (s: B.lbuffer U32.t 5)
+  (wrap: I32.t)
+  (uncompressed: Seq.seq U8.t) =
+  let s' = B.as_seq h s in
+  let len = Seq.length uncompressed in
+  (I32.v wrap == 1 ==>
+    Adler32.adler32_matched #len uncompressed (adler s')) /\
+  ((CFlags.gzip == true /\ I32.v wrap == 2) ==>
+    CRC32.crc32_matched len uncompressed (adler s') true)
+
+let stream_valid
+  (h: HS.mem)
+  (s: B.lbuffer U32.t 5)
+  (next_in: B.pointer (B.buffer U8.t))
+  (next_out: B.pointer (B.buffer U8.t))
+  (wrap: I32.t)
+  (uncompressed: Seq.seq U8.t) =
+  let s' = B.as_seq h s in
+  let len = Seq.length uncompressed in
+  let next_out' = B.get h next_out 0 in
+  let next_in' = B.get h next_in 0 in
+  B.live h s /\
+  B.disjoint next_in next_out /\
+  B.disjoint next_in next_out' /\
+  B.disjoint next_in' next_out /\
+  B.disjoint next_in' next_out' /\
+
+  next_in_valid h s next_in /\ next_out_valid h s next_out /\
+  adler_valid h s wrap uncompressed
